theories/Semantics/IMP/Syntax.v
@@ -1,8 +1,12 @@
 From stdpp Require Import prelude.
 
+Section sec_syntax.
+
+Context (L : Type).
+
 Inductive AExp : Type :=
     | AVal : Z -> AExp
-    | Var : nat -> AExp
+    | Var : L -> AExp
     | Plus : AExp -> AExp -> AExp
     | Minus : AExp -> AExp -> AExp
     | Mul : AExp -> AExp -> AExp.
@@ -17,7 +21,28 @@ Inductive BExp : Type :=
 
 Inductive Cmd : Type :=
     | Skip : Cmd
-    | Asgn : nat -> AExp -> Cmd
+    | Asgn : L -> AExp -> Cmd
     | Seq : Cmd -> Cmd -> Cmd
     | If : BExp -> Cmd -> Cmd -> Cmd
     | While : BExp -> Cmd -> Cmd.
+
+End sec_syntax.
+
+Arguments AVal {L}%type_scope _%Z_scope : assert.
+Arguments Var {L}%type_scope _ : assert.
+Arguments Plus {L}%type_scope _ _ : assert.
+Arguments Minus {L}%type_scope _ _ : assert.
+Arguments Mul {L}%type_scope _ _ : assert.
+
+Arguments BVal {L}%type_scope _%bool_scope : assert.
+Arguments AEq {L}%type_scope _ _ : assert.
+Arguments ALe {L}%type_scope _ _ : assert.
+Arguments Not {L}%type_scope _ : assert.
+Arguments And {L}%type_scope _ _ : assert.
+Arguments Or {L}%type_scope _ _ : assert.
+
+Arguments Skip {L}%type_scope : assert.
+Arguments Asgn {L}%type_scope _ _ : assert.
+Arguments Seq {L}%type_scope _ _ : assert.
+Arguments If {L}%type_scope _ _ _ : assert.
+Arguments While {L}%type_scope _ _ : assert.
