theories/Semantics/IMP/Eval.v
@@ -2,8 +2,12 @@ From stdpp Require Import prelude.
 
 From Semantics Require Import Syntax State.
 
-Definition aeval (sigma : State) : AExp -> Z :=
-    fix eval (a : AExp) :=
+Section sec_eval.
+
+Context `{EqDecision L}.
+
+Definition aeval (sigma : State L) : AExp L -> Z :=
+    fix eval (a : AExp L) :=
     match a with
     | AVal n => n
     | Var x => sigma x
@@ -13,8 +17,8 @@ Definition aeval (sigma : State) : AExp -> Z :=
     end.
 
 
-Definition beval (sigma : State) : BExp -> bool :=
-    fix eval (b : BExp) :=
+Definition beval (sigma : State L) : BExp L -> bool :=
+    fix eval (b : BExp L) :=
     match b with
     | BVal b => b
     | AEq a1 a2 => bool_decide (aeval sigma a1 = aeval sigma a2)
@@ -23,3 +27,5 @@ Definition beval (sigma : State) : BExp -> bool :=
     | And b1 b2 => andb (eval b1) (eval b2)
     | Or b1 b2 => orb (eval b1) (eval b2)
     end.
+
+End sec_eval.
